theorems/Utils.v
@@ -1,6 +1,0 @@
-Inductive Result (T: Type) (E: Type): Type :=
-	| Ok (value: T)
-	| Err (error: E).
-
-Arguments Ok {T} {E} _.
-Arguments Err {T} {E} _.
